importing Nik's example from nik_setoids

examples/rel/Setoids.Example.fst
@@ -1,44 +1,45 @@
 module Setoids.Example
+#set-options "--max_fuel 0 --initial_ifuel 1 --max_ifuel 1"
 
 open Setoids
-
 module DM = FStar.DependentMap
 
 /// Some basic functions and the same effect as for the crypto example, but without random tape.
 
-let option_rel (#a:Type) (arel:rel a) =
+let option_rel (#a:Type) (arel:erel a) : erel (option a) =
   fun (x:option a) (y:option a) ->
     match x,y with
-    | None,None -> True // <: prop
-    | Some some_x, Some some_y -> (arel some_y some_x) // <: prop
-    | _, _ -> False // <: prop
+    | None,None -> True
+    | Some some_x, Some some_y -> (arel some_y some_x)
+    | _, _ -> False
 
-let eff (#s:Type) (#a:Type) (srel:rel s) (arel:rel a) =
+let eff (#s:Type) (#a:Type) (srel:erel s) (arel:erel a) =
   srel ^--> ((option_rel arel) ** srel)
 
-#set-options "--z3rlimit 150 --query_stats"
 let eff_rel #s #a
     (srel: erel s)
     (arel: erel a)
     : erel (eff srel arel)
-  = arrow_rel srel ((option_rel #a arel) ** srel)
+  = e_arrow_rel srel ((option_rel #a arel) ** srel)
 
 /// returning a result into a computation
+unfold
 let return (#s:Type) (#a:Type) (#srel:erel s) (#arel:erel a) (x:a)
   : eff #s #a srel arel
   = fun s0 -> Some x, s0
 
-let lift_left (#s1:Type) (#s1rel:erel s1{lo s1 == s1rel}) #s2 (#s2rel:erel s2) #a (#arel:erel a) (f:eff s1rel arel)
-  : ((s1rel ** s2rel) ^--> ((option_rel arel) ** (s1rel ** s2rel)))
+unfold
+let lift_left (#s1:Type) (#s1rel:erel s1) #s2 (#s2rel:erel s2) #a (#arel:erel a) (f:eff s1rel arel)
+  : eff (s1rel ** s2rel) arel
   = fun (s1, s2) ->
       match f s1 with
       | None, s1' ->
         None, (s1', s2)
-
       | Some x, s1' ->
         Some x, (s1', s2)
 
-let lift_right #s1 (#s1rel:erel s1) #s2 (#s2rel:erel s2{s2rel == lo s2}) #a (#arel:erel a) (f:eff s2rel arel)
+unfold
+let lift_right #s1 (#s1rel:erel s1) #s2 (#s2rel:erel s2) #a (#arel:erel a) (f:eff s2rel arel)
   : eff (s1rel ** s2rel) arel
   = fun (s1, s2) ->
       match f s2 with
@@ -46,7 +47,7 @@ let lift_right #s1 (#s1rel:erel s1) #s2 (#s2rel:erel s2{s2rel == lo s2}) #a (#ar
       | Some x, s2' -> Some x, (s1, s2')
 
 /// sequential composition of `eff` computations
-#set-options "--z3rlimit 150 --max_fuel 0 --max_ifuel 2 --query_stats"
+unfold
 let bind #s #a (#srel:erel s) (#arel:erel a) #b (#brel:erel b)
          ($f:eff #s #a srel arel)
          (g:arel ^--> eff_rel #s #b srel brel)
@@ -59,14 +60,16 @@ let bind #s #a (#srel:erel s) (#arel:erel a) #b (#brel:erel b)
        None, s1
 
 /// reading the entire state
+unfold
 let get #s (#srel:erel s) : eff srel srel =
   fun s0 -> Some s0, s0
 
 /// writing the entire state
+unfold
 let put #s (#srel:erel s) : (srel ^--> eff_rel srel (lo unit)) =
   fun s _ -> Some (), s
 
-let get_oracle #sig (m:module_t sig) (o:sig.labels) : sig.ops o = DM.sel m o
+let get_oracle #sig (l:sig.labels) : (sig_rel sig ^--> sig.rels l) = fun m -> DM.sel m l
 
 /// Examples of simple module compositions using the simple state monad
 /// introduced in the Setoids package.
@@ -77,7 +80,7 @@ let get_oracle #sig (m:module_t sig) (o:sig.labels) : sig.ops o = DM.sel m o
 /// the integer contained in the integer container.
 
 let int_container_st = int
-let int_container_state_rel = lo int
+let int_container_state_rel : erel _ = lo int
 
 let get_int_t = lo unit ^--> eff_rel int_container_state_rel (lo int)
 let get_int :get_int_t =
@@ -88,7 +91,6 @@ let get_int :get_int_t =
 type int_container_labels =
   | GET
 
-#set-options "--z3rlimit 350 --max_fuel 0 --max_ifuel 1"
 let int_container_field_types : int_container_labels -> Type =
     function GET -> get_int_t
 
@@ -116,9 +118,9 @@ let int_container_functor
 
 /// The eq_checker has no state.
 let eq_checker_st = unit
-let eq_checker_state_rel = lo unit
+let eq_checker_state_rel : erel _ = lo unit
 
-let combined_state_rel = int_container_state_rel ** eq_checker_state_rel
+let combined_state_rel : erel _ = int_container_state_rel ** eq_checker_state_rel
 
 /// In order for two modules to be composed, every function needs to get an
 /// instance of a module with the desired signature as input. However, we don't
@@ -130,21 +132,105 @@ let combined_state_rel = int_container_state_rel ** eq_checker_state_rel
 /// thing).
 let is_eq_t = ((sig_rel int_container_sig) ** lo int) ^--> eff_rel combined_state_rel (lo bool)
 let is_eq_t_trunc = (lo int) ^--> eff_rel combined_state_rel (lo bool)
+let ( ^^--> ) (#a:Type) (#b:Type) (arel:rel a) (brel:rel b) =
+  f:(a -> b)
+let is_eq_t_base = ((sig_rel int_container_sig) ** lo int) ^^--> eff_rel combined_state_rel (lo bool)
 
-let is_eq  : is_eq_t =
-  fun (ih,x) ->
-    let get_int : get_int_t = get_oracle ih GET in
-    st <--
-      lift_left
-      (get_int ());
-    return (st = x)
+let is_eq'  : is_eq_t_base =
+  fun (ih, x) ->
+    ((let get_int : get_int_t = get_oracle GET ih in
+     ((st <-- lift_left (get_int ());
+       return (x = st)) <: eff combined_state_rel (lo bool))))
+
+let _goes_through_easily (a0 a1:type_of (sig_rel int_container_sig))
+                         (s0 s1:type_of int_container_state_rel)
+  : Lemma
+      (requires
+        a0 `(sig_rel int_container_sig)` a1 /\
+        s0 `int_container_state_rel` s1)
+      (ensures (
+        let g0 : get_int_t = get_oracle GET a0 in
+        let g1 : get_int_t = get_oracle GET a1 in
+        g0 () s0 == g1 () s1))
+  = ()
+
+#set-options "--max_fuel 0 --initial_ifuel 1 --max_ifuel 1 --z3rlimit 50 --__temp_no_proj Setoids.Example --query_stats"
+let _goes_through_easily' (module_sig:sig)
+                          (state_t:Type)
+                          (state_rel:erel Type)
+                          (input_t:Type)
+                          (input_rel:erel input_t{input_rel == lo input_t})
+                          (output_t:Type)
+                          (output_rel:erel output_t{output_rel == lo output_t})
+                          (label:module_sig.labels{Mksig?.ops module_sig label == (input_rel ^--> eff_rel state_rel output_rel)})
+                          (a0 a1:type_of (sig_rel module_sig))
+                          (s0 s1:type_of state_rel)
+                          (x0 x1:type_of (input_rel))
+  : Lemma
+      (requires
+        a0 `(sig_rel module_sig)` a1 /\
+        s0 `state_rel` s1 /\
+        x0 `input_rel` x1)
+      (ensures (
+        let g0 : (input_rel ^--> eff_rel state_rel output_rel) = get_oracle #module_sig label (fst a0) in
+        let g1 : (input_rel ^--> eff_rel state_rel output_rel) = get_oracle #module_sig label (fst a1) in
+        (g0 x0 s0) == g1 x1 s1))
+  = ()
+
+#set-options "--max_fuel 0 --initial_ifuel 1 --max_ifuel 1 --z3rlimit 50 --__temp_no_proj Setoids.Example --query_stats"
+val get_related (state_t:Type)
+                (state_rel:erel state_t{state_rel == lo state_t})
+                (input_t:Type)
+                (input_rel:erel input_t{input_rel == lo input_t})
+                (output_t:Type)
+                (output_rel:erel output_t{output_rel == lo output_t})
+                (other_state_t:Type)
+                (other_state_rel:erel other_state_t{other_state_rel == lo other_state_t})
+                (module_sig:sig)
+                (label:module_sig.labels{Mksig?.ops module_sig label == (input_rel ^--> eff_rel state_rel output_rel)})
+                (a0 a1:type_of (sig_rel module_sig ** output_rel))
+                (s0 s1:type_of (state_rel ** other_state_rel))
+                (x0 x1:type_of (input_rel))
+  : Lemma
+      (requires
+        a0 `((sig_rel module_sig) ** output_rel)` a1 /\
+        Mksig?.ops module_sig label == input_t -> state_t -> output_t /\
+        s0 `(state_rel ** other_state_rel)` s1)
+      (ensures (
+        let g0 : (input_rel ^--> eff_rel state_rel output_rel) = get_oracle #module_sig label (fst a0) in
+        let g1 : (input_rel ^--> eff_rel state_rel output_rel) = get_oracle #module_sig label (fst a1) in
+        let g00 : (eff (state_rel ** other_state_rel) (output_rel)) = lift_left (g0 x0 <: eff state_rel (output_rel)) in
+        let g11 : (eff (state_rel ** other_state_rel) (output_rel)) = lift_left (g1 x1 <: eff state_rel (output_rel)) in
+        (g00 s0) == (g11 s1)))
+let get_related state_t state_rel input_t input_rel output_t output_rel other_state_t other_state_rel module_sig label a0 a1 s0 s1 x0 x1 =
+    let g0 : (input_rel ^--> eff_rel (state_rel) (output_rel)) = get_oracle #module_sig label (fst a0) in
+    let g1 : (input_rel ^--> eff_rel (state_rel) (output_rel)) = get_oracle #module_sig label (fst a1) in
+    let g00 : (eff (state_rel ** other_state_rel) (output_rel)) = lift_left (g0 x0 <: eff state_rel (output_rel)) in
+    let g11 : (eff (state_rel ** other_state_rel) (output_rel)) = lift_left (g1 x1 <: eff state_rel (output_rel)) in
+    //let g0' : (input_rel ^--> eff_rel (state_rel) (output_rel)) = fun x -> g0 x (fst s0)
+    assert((g0 x0 (fst s0)) `((option_rel output_rel) ** (state_rel))` (g1 x1 (fst s1)))
+
+let is_eq : is_eq_t =
+  let aux (a0 a1:type_of ((sig_rel int_container_sig) ** lo int))
+          (s0 s1:type_of combined_state_rel)
+  : Lemma
+      (requires
+        a0 `((sig_rel int_container_sig) ** lo int)` a1 /\
+        s0 `combined_state_rel` s1)
+      (ensures
+        (is_eq' a0 s0 `((option_rel (lo bool)) ** combined_state_rel)`
+         is_eq' a1 s1))
+     [SMTPat (is_eq' a0 s0);
+      SMTPat (is_eq' a1 s1)]
+  = get_related eq_checker_st eq_checker_state_rel a0 a1 s0 s1
+ in
+ is_eq'
 
 type eq_checker_labels =
   | IS_EQ
 
-#set-options "--z3rlimit 350 --max_fuel 0 --max_ifuel 1"
 let eq_checker_field_types : eq_checker_labels -> Type =
-    function  IS_EQ -> is_eq_t_trunc
+  function  IS_EQ -> is_eq_t_trunc
 
 let eq_checker_field_rels : (l:eq_checker_labels -> erel (eq_checker_field_types l)) =
   function
@@ -159,11 +245,43 @@ let eq_checker_sig = {
     rels = eq_checker_field_rels
   }
 
-#set-options "--z3rlimit 350 --max_fuel 0 --max_ifuel 0"
-#set-options "--query_stats"
-let eq_checker_functor
-  : functor_t (int_container_sig) (eq_checker_sig)
+let eq_checker_functor'
+  : module_t int_container_sig -> module_t eq_checker_sig
   = fun ih ->
       let is_eq' : is_eq_t_trunc = fun x -> is_eq (ih,x) in
       let m : module_t (eq_checker_sig) = DM.create #_ #(eq_checker_sig).ops (function IS_EQ -> is_eq') in
-      admit()
+      m
+
+let eq_checker_functor
+  : functor_t int_container_sig eq_checker_sig
+  =
+    let intro_eq_checker (i0 i1:module_t int_container_sig)
+      : Lemma
+        (requires
+          i0 `sig_rel int_container_sig` i1)
+        (ensures
+          eq_checker_functor' i0 `sig_rel eq_checker_sig` eq_checker_functor' i1)
+        [SMTPat (eq_checker_functor' i0);
+         SMTPat (eq_checker_functor' i1)]
+    = let m0 = eq_checker_functor' i0 in
+      let m1 = eq_checker_functor' i1 in
+      let is_eq_0 : is_eq_t_trunc = get_oracle IS_EQ m0 in
+      let is_eq_1 : is_eq_t_trunc = get_oracle IS_EQ m1 in
+      let aux (v0 v1:int) (s0 s1:_)
+        : Lemma
+          (requires
+             v0 `lo int` v1 /\
+             s0 `combined_state_rel` s1)
+          (ensures
+             is_eq_0 v0 s0
+               `(option_rel (lo bool) ** combined_state_rel)`
+             is_eq_1 v1 s1)
+          [SMTPat (is_eq_0 v0 s0);
+           SMTPat (is_eq_1 v1 s1)]
+        = assert (is_eq_0 v0 s0 == is_eq (i0, v0) s0);
+          assert (is_eq_1 v1 s1 == is_eq (i1, v1) s1);
+          assert ((i0, v0) `(sig_rel int_container_sig ** lo int)` (i1, v1))
+      in
+      ()
+    in
+    eq_checker_functor'
